PrimParser/Basic.lean
@@ -366,6 +366,9 @@ instance : GradedApplicative (Parser σ τ ε) where
 instance : GradedMonad (Parser σ τ ε) where
   gbind := bind
 
+theorem gmap_run (f : α → β) (p : Parser σ τ ε g α) (t : Input σ τ n)
+  : (f <$>ᵍ p).run t = f <$> p.run t := rfl
+
 theorem gbind_run (m : Parser σ τ ε g α) (k : α → Parser σ τ ε g' β) (t : Input σ τ n)
   : (m >>=ᵍ k).run t
     = (m.run t).handle (m.sound t) (fun _ x => x.bindParser t k) (fun _ e => failure e) := rfl
@@ -823,6 +826,9 @@ def count1
       let rest ← count1 n p
       return (x ::ᵥ rest)
       grade_by by simp
+
+theorem count1_succ (n : Nat) (p : Parser σ τ ε conditional α)
+  : count1 (n + 1) p = (p >>=ᵍ fun x => count1 n p >>=ᵍ fun rest => gpure (x ::ᵥ rest)) := rfl
 
 /-- Parse exactly `n` occurrences of `p`. -/
 def count
