PrimParser/BytesWindow.lean
@@ -1,0 +1,40 @@
+/-!
+# A window of a `ByteArray`.
+-/
+
+namespace Parser
+
+/-- A `w` bytes window of `buf[start .. start + w - 1]` -/
+structure BytesWindow (w : Nat) where
+  buf : ByteArray
+  start : Nat
+  valid : start + w ≤ buf.size
+
+variable
+  {w : Nat}
+
+instance : GetElem (BytesWindow w) Nat UInt8 (fun _ i => i < w) where
+  getElem b i h := b.buf[b.start + i]'(by have := b.valid; omega)
+
+@[simp] theorem BytesWindow.getElem_def (b : BytesWindow w) (i : Nat) (h : i < w)
+  : b[i] = b.buf[b.start + i]'(by have := b.valid; omega) := rfl
+
+abbrev BytesWindow.narrow
+  (b : BytesWindow w)
+  (offset w' : Nat)
+  (h : offset + w' ≤ w := by omega) : BytesWindow w' where
+  buf := b.buf
+  start := b.start + offset
+  valid := by have := b.valid; omega
+
+def BytesWindow.toByteArray (b : BytesWindow w) : ByteArray :=
+  b.buf.extract b.start (b.start + w)
+
+theorem BytesWindow.toByteArray_succ (b : BytesWindow (w + 1))
+  : b.toByteArray = [b[0]].toByteArray ++ (b.narrow 1 w).toByteArray := by
+  have := b.valid
+  simp [toByteArray, getElem_def]
+  rw [← ByteArray.extract_add_one (i := b.start) (by omega), ByteArray.extract_append_extract]
+  congr <;> omega
+
+end Parser
