Tests.lean
@@ -6,3 +6,4 @@ import Tests.Examples.Json
 import Tests.Examples.SExp
 import Tests.Examples.Lambda
 import Tests.Examples.Lexer
+import Tests.Byte
